ERT/Higher/Typed/Wk.lean
@@ -1,37 +1,39 @@
 import ERT.Higher.Typed.Basic
 
+--TODO: Port to version from weakening utils
+
 namespace HERT
 
-inductive WkCtx {α}: (ℕ -> ℕ) -> (Γ: List (Var α)) -> (Δ: List (Var α)) -> Type
+inductive WkCtx: (ℕ -> ℕ) -> (Γ: List Var) -> (Δ: List Var) -> Type
   | nil (ρ): WkCtx ρ [] []
   | lift (A): WkCtx ρ Γ Δ -> w'.le w →
     WkCtx (liftWk ρ) (Var.mk (A.wk ρ) w :: Γ) (Var.mk A w' :: Δ)
   | step (A): WkCtx ρ Γ Δ -> WkCtx (stepWk ρ) (Var.mk A w :: Γ) Δ
 
-def WkCtx.slift {α ρ Γ Δ} (A w) (R: @WkCtx α ρ Γ Δ):
+def WkCtx.slift {ρ Γ Δ} (A w) (R: @WkCtx ρ Γ Δ):
   WkCtx (liftWk ρ) (Var.mk (A.wk ρ) w :: Γ) (Var.mk A w :: Δ) :=
   WkCtx.lift _ R (World.le.refl _)
 
-def WkCtx.src {α ρ Γ Δ} (_: @WkCtx α ρ Γ Δ): List (Var α) := Γ
-def WkCtx.trg {α ρ Γ Δ} (_: @WkCtx α ρ Γ Δ): List (Var α) := Δ
+def WkCtx.src {ρ Γ Δ} (_: @WkCtx ρ Γ Δ): List Var := Γ
+def WkCtx.trg {ρ Γ Δ} (_: @WkCtx ρ Γ Δ): List Var := Δ
 
-def WkCtx.ix {α ρ Γ Δ} (_: @WkCtx α ρ Γ Δ): ℕ -> ℕ := ρ
+def WkCtx.ix {ρ Γ Δ} (_: @WkCtx ρ Γ Δ): ℕ -> ℕ := ρ
 
-def HasVar.wk {α ρ Γ Δ A n w}: @WkCtx α ρ Γ Δ -> HasVar Δ n A w -> HasVar Γ (ρ n) (A.wk ρ) w
+def HasVar.wk {ρ Γ Δ A n w}: @WkCtx ρ Γ Δ -> HasVar Δ n A w -> HasVar Γ (ρ n) (A.wk ρ) w
   | WkCtx.lift _ ρ H', head _ _ H => Term.wk_lift_succ _ _ ▸ head _ _ (H.trans H')
   | WkCtx.lift _ ρ _, tail v => Term.wk_lift_succ _ _ ▸ tail (v.wk ρ)
   | WkCtx.step _ ρ, v => Term.wk_step_succ _ _ ▸ tail (v.wk ρ)
 
-theorem Term.IsSort.fv_zero {α K w} (H: @IsSort α K w): K.fv = 0 := by cases H <;> rfl
+theorem Term.IsSort.fv_zero {K w} (H: @IsSort K w): K.fv = 0 := by cases H <;> rfl
 
-theorem Term.IsSort.eq_wk {α K w} (H: @IsSort α K w) (ρ: _): K.wk ρ = K := K.wk_closed (H.fv_zero)
+theorem Term.IsSort.eq_wk {K w} (H: @IsSort K w) (ρ: _): K.wk ρ = K := K.wk_closed (H.fv_zero)
 
-theorem Term.IsSort.eq_wk' {α K w} (H: @IsSort α K w) (ρ ρ': _): K.wk ρ = K.wk ρ' :=
+theorem Term.IsSort.eq_wk' {K w} (H: @IsSort K w) (ρ ρ': _): K.wk ρ = K.wk ρ' :=
   (H.eq_wk ρ).trans (H.eq_wk ρ').symm
 
-def Term.IsSort.wk {α K w} (H: @IsSort α K w) (ρ: _): IsSort (K.wk ρ) w := (H.eq_wk _).symm ▸ H
+def Term.IsSort.wk {K w} (H: @IsSort K w) (ρ: _): IsSort (K.wk ρ) w := (H.eq_wk _).symm ▸ H
 
-def Term.HasType.wk {α ρ Γ Δ a A w} (R: @WkCtx α ρ Γ Δ)
+def Term.HasType.wk {ρ Γ Δ a A w} (R: @WkCtx ρ Γ Δ)
   : HasType Δ a A w -> HasType Γ (a.wk ρ) (A.wk ρ) w
   | var v HA HS => var (v.wk R) (HA.wk R) (HS.wk ρ)
   | pi HA HKA HB HKB =>
