ERT/Abstract/Simple.lean
@@ -1,0 +1,14 @@
+import ERT.Abstract.Basic
+
+namespace Abstract
+
+class SimplyTyped.{w} (α: Type u) (τ: outParam (Type v)) extends Syntax α where
+  wellTyped: (a: α)
+    -> (Fin (arity a) -> τ)
+    -> ((i: Fin (arity a)) -> (Fin (binding a i)) -> τ)
+    -> τ
+    -> Sort w
+
+structure Ctx (τ) where
+  len: ℕ
+  types: Fin len -> τ
