ERT/Higher/Typed/Ctx.lean
@@ -4,15 +4,15 @@ namespace HERT
 
 open World
 
-structure Var (α) where
-  ty: Term α
+structure Var where
+  ty: Term
   world: World
 
-structure Var.le {α} (x y: Var α): Prop where
+structure Var.le (x y: Var): Prop where
   ty: x.ty = y.ty
   world: x.world ≤ y.world
 
-instance Var.instPartialOrder {α}: PartialOrder (Var α) where
+instance Var.instPartialOrder: PartialOrder (Var) where
   le := le
   le_refl _ := ⟨rfl, le_refl _⟩
   le_trans _ _ _ l r := ⟨l.ty.trans r.ty, le_trans l.world r.world⟩
@@ -20,10 +20,10 @@ instance Var.instPartialOrder {α}: PartialOrder (Var α) where
   | ⟨_, _⟩,  ⟨_, _⟩, l, r
     => by rw [Var.mk.injEq]; exact ⟨l.ty, le_antisymm l.world r.world⟩
 
-inductive HasVar {α}: List (Var α) -> ℕ -> Term α -> World -> Type where
+inductive HasVar: List (Var) -> ℕ -> Term -> World -> Type where
   | head: ∀ {w w'} (Γ A), w'.le w -> HasVar (Var.mk A w :: Γ) 0 (A.wk Nat.succ) w'
   | tail: ∀ {Γ A v n w}, HasVar Γ n A w -> HasVar (v :: Γ) (n + 1) (A.wk Nat.succ) w
 
-def HasVar.toGhost {α Γ n A w}: @HasVar α Γ n A w -> HasVar Γ n A ghost
+def HasVar.toGhost {Γ n A w}: @HasVar Γ n A w -> HasVar Γ n A ghost
   | head _ _A _ => head _ _ (World.le.ghost _)
   | tail H => tail H.toGhost
